Factor out hoare logic experiments

theories/Context.v
@@ -6,8 +6,6 @@ Require Blech.OptionNotations.
 Require Import Coq.Unicode.Utf8.
 Require Import Coq.Classes.SetoidClass.
 Require Coq.Lists.List.
-Require Import Coq.Logic.FunctionalExtensionality.
-Require Import Coq.Logic.PropExtensionality.
 
 Require Import FunInd.
 
@@ -332,64 +330,6 @@ Proof using.
   subst.
   auto.
 Defined.
-
-(* FIXME put elsewhere/make a monad? *)
-Section Heap.
-  Context {A: Type}.
-
-  Definition hprop := A → store → Prop.
-
-  Inductive hempty: hprop :=
-  | hempty_intro {a}: hempty a Map.empty.
-
-  Inductive hpure P: hprop :=
-  | hpure_intro {a}: P → hpure P a Map.empty.
-
-  Inductive hsingle X N: hprop :=
-  | hsingle_intro {a}: hsingle X N a (Map.one X N).
-
-  Inductive hstar (H H': hprop): hprop :=
-  | hstar_intro {a h1 h2}:
-    H a h1 → H' a h2 → Map.disjoint h1 h2 →
-    hstar H H' a (Map.merge h1 h2).
-  Inductive hexists {A} (J: A → hprop): hprop :=
-  | hexists_intro {x a h}: J x a h → hexists J a h.
-End Heap.
-
-Arguments hprop: clear implicits.
-
-Notation "\[]" := hempty (at level 0).
-Notation "\[ P ]" := (hpure P) (at level 0, format "\[ P ]").
-Notation "p '~~>' v" := (hsingle p v) (at level 32).
-Notation "H1 '\*' H2" := (hstar H1 H2) (at level 41, right associativity).
-
-Notation "'\exists' x1 .. xn , H" :=
-  (hexists (λ x1, .. (hexists (λ xn, H)) ..))
-    (at level 39, x1 binder, H at level 50, right associativity,
-      format "'[' '\exists' '/ ' x1 .. xn , '/ ' H ']'").
-
-Definition ig {A} (P: hprop unit): hprop A := λ _, P tt.
-
-Theorem hstar_assoc:
-  ∀ {V} {A B C: hprop V},
-    (A \* B) \* C = A \* (B \* C).
-Proof using.
-  admit.
-Admitted.
-
-(* Satisfaction defines a sort of nondeterministic Hoare logic *)
-
-(* based on https://softwarefoundations.cis.upenn.edu/slf-current/Hprop.html *)
-Inductive eval: context → store → normal → store → Prop :=
-| eval_sat {E σ σ' N}: sat σ' E N → eval E σ N (Map.merge σ σ').
-
-Definition hoare E (H: hprop unit) (Q: hprop normal): Prop :=
-  ∀ s,
-    H tt s →
-    ∃ s' N, eval E s N s' /\ Q N s'.
-
-Definition triple E H (Q: hprop normal) : Prop :=
-  ∀ H', hoare E (H \* H') (Q \* ig H').
 
 Definition oftype t := { E | Map.empty ⊢ E ? t }.
 
