theories/Hoare.v
@@ -1,0 +1,108 @@
+Require Blech.Map.
+Require Import Blech.Spec.
+Require Import Blech.SpecNotations.
+
+Require Import Coq.Unicode.Utf8.
+Require Coq.Lists.List.
+Require Import Coq.Logic.FunctionalExtensionality.
+Require Import Coq.Logic.PropExtensionality.
+
+Import IfNotations.
+
+Implicit Type Δ: linear.
+Implicit Type E: context.
+Implicit Type t: type.
+Implicit Type N: normal.
+Implicit Types X Y: cvar.
+Implicit Type σ: store.
+
+Import Map.MapNotations.
+
+(* Satisfaction defines a sort of nondeterministic Hoare logic *)
+
+(* based on https://softwarefoundations.cis.upenn.edu/slf-current/Hprop.html *)
+
+(* FIXME make a monad? *)
+Section Heap.
+  Context {A: Type}.
+
+  Definition hprop := A → store → Prop.
+
+  Inductive hempty: hprop :=
+  | hempty_intro {a}: hempty a Map.empty.
+
+  Inductive hpure P: hprop :=
+  | hpure_intro {a}: P → hpure P a Map.empty.
+
+  Inductive hsingle X N: hprop :=
+  | hsingle_intro {a}: hsingle X N a (Map.one X N).
+
+  Inductive hstar (H H': hprop): hprop :=
+  | hstar_intro {a h1 h2}:
+    H a h1 → H' a h2 → Map.disjoint h1 h2 →
+    hstar H H' a (Map.merge h1 h2).
+  Inductive hexists {A} (J: A → hprop): hprop :=
+  | hexists_intro {x a h}: J x a h → hexists J a h.
+End Heap.
+
+Arguments hprop: clear implicits.
+
+Notation "\[]" := hempty (at level 0).
+Notation "\[ P ]" := (hpure P) (at level 0, format "\[ P ]").
+Notation "p '~~>' v" := (hsingle p v) (at level 32).
+Notation "H1 '\*' H2" := (hstar H1 H2) (at level 41, right associativity).
+
+Notation "'\exists' x1 .. xn , H" :=
+  (hexists (λ x1, .. (hexists (λ xn, H)) ..))
+    (at level 200, x1 binder, H at level 50, right associativity,
+      format "'[' '\exists' '/ ' x1 .. xn , '/ ' H ']'").
+
+Definition ig {A} (P: hprop unit): hprop A := λ _, P tt.
+
+Lemma disjointness {h0 h1 h2: store}:
+    Map.disjoint h1 h0 → Map.disjoint (h1 ∪ h0) h2 →
+    Map.disjoint h0 h2.
+Proof.
+  unfold Map.disjoint.
+  intros p q.
+  intro k.
+  destruct (p k).
+  all: auto.
+  destruct (q k).
+  all: auto.
+  rewrite Map.find_merge_r in H0.
+  all: auto.
+Qed.
+
+Theorem hstar_assoc:
+  ∀ {V} {A B C: hprop V},
+    (A \* B) \* C = A \* (B \* C).
+Proof using.
+  intros.
+  extensionality v.
+  extensionality σ.
+  apply propositional_extensionality.
+  split.
+  - intro p.
+    destruct p.
+    destruct H.
+    rewrite Map.merge_assoc.
+    constructor.
+    1: auto.
+    1: constructor.
+    all: auto.
+    + eapply disjointness.
+      all: eauto.
+    + admit.
+Admitted.
+
+Inductive eval: context → store → normal → store → Prop :=
+| eval_sat {E σ σ' N}: sat σ' E N → eval E σ N (Map.merge σ σ').
+
+Definition hoare E (H: hprop unit) (Q: hprop normal): Prop :=
+  ∀ s,
+    H tt s →
+    ∃ s' N, eval E s N s' /\ Q N s'.
+
+Definition triple E H (Q: hprop normal) : Prop :=
+  ∀ H', hoare E (H \* H') (Q \* ig H').
